theories/L/Complexity/Cook/FSAT_to_SAT.v
@@ -14,10 +14,59 @@ Definition tseytinOr (v v1 v2 : var) : cnf :=
 Definition tseytinNot (v v' : var) : cnf := 
   [[(false, v); (false, v')]; [(true, v); (true, v')]].
 
+Lemma tseytinAnd_sat a v v1 v2 : satisfies a (tseytinAnd v v1 v2) <-> (evalVar a v = true <-> (evalVar a v1 = true /\ evalVar a v2 = true)). 
+Proof. 
+  unfold tseytinAnd, satisfies. 
+  destruct (evalVar a v) eqn:H1, (evalVar a v1) eqn:H2, (evalVar a v2) eqn:H3; cbn in *;
+    repeat (first [rewrite H1  | rewrite H2 | rewrite H3 ]; cbn ); tauto. 
+Qed. 
+
+Lemma tseytinOr_sat a v v1 v2 : satisfies a (tseytinOr v v1 v2) <-> (evalVar a v = true <-> (evalVar a v1 = true \/ evalVar a v2 = true)). 
+Proof. 
+  unfold tseytinOr, satisfies. 
+  destruct (evalVar a v) eqn:H1, (evalVar a v1) eqn:H2, (evalVar a v2) eqn:H3; cbn in *;
+    repeat (first [rewrite H1  | rewrite H2 | rewrite H3 ]; cbn ); tauto. 
+Qed. 
+
+Lemma tseytinNot_sat a v v': satisfies a (tseytinNot v v') <-> (evalVar a v = true <-> not (evalVar a v' = true)). 
+Proof. 
+  unfold tseytinNot, satisfies. 
+  destruct (evalVar a v) eqn:H1, (evalVar a v') eqn:H2; cbn in *;
+    repeat (first [rewrite H1  | rewrite H2]; cbn );
+  (split; [intros H; try congruence; split; intros; congruence | tauto]).
+Qed.
+
+Lemma tseytinAnd_varBound v v1 v2 : varBound_cnf (S (Nat.max v (Nat.max v1 v2))) (tseytinAnd v v1 v2). 
+Proof. 
+  unfold tseytinAnd. repeat match goal with 
+    | [ |- varBound_clause _ _] => constructor 
+    | [ |- varBound_cnf _ _ ] => constructor
+    | _ => lia
+  end. 
+Qed. 
+
+Lemma tseytinOr_varBound v v1 v2 : varBound_cnf (S (Nat.max v (Nat.max v1 v2))) (tseytinOr v v1 v2). 
+Proof. 
+  unfold tseytinOr. repeat match goal with 
+    | [ |- varBound_clause _ _] => constructor 
+    | [ |- varBound_cnf _ _ ] => constructor
+    | _ => lia
+  end. 
+Qed. 
+
+Lemma tseytinNot_varBound v v' : varBound_cnf (S (Nat.max v v')) (tseytinNot v v'). 
+Proof. 
+  unfold tseytinNot. repeat match goal with 
+    | [ |- varBound_clause _ _] => constructor 
+    | [ |- varBound_cnf _ _ ] => constructor
+    | _ => lia
+  end. 
+Qed. 
+
 Fixpoint tseytin' (nfVar : var) (f : formula) : (var * cnf * var) := 
   match f with 
-  | Ftrue => (nfVar, [[nfVar]], S nfVar)
-  | Fvar v => (v, [[]], nfVar)
+  | Ftrue => (nfVar, [[(true, nfVar)]], S nfVar)
+  | Fvar v => (v, [], nfVar)
   | For f1 f2 => let
       '(rv1, N1, nfVar1) := tseytin' nfVar f1 in let 
       '(rv2, N2, nfVar2) := tseytin' nfVar1 f2 in 
@@ -32,10 +81,73 @@ Fixpoint tseytin' (nfVar : var) (f : formula) : (var * cnf * var) :=
   end. 
 
 Definition tseytin f : var * cnf := 
-  let '(repVar, N, _) := tseytin' (S (formula_maxVar f)) f in (repVar, N). 
+  let '(repVar, N, _) := tseytin' (formula_maxVar f) f in (repVar, N). 
 
 (*a variable v represents a formula f with respect to a CNF N iff the CNF with the variable v assumed to be true is equisatisfiable to f*)
 Definition formula_repr (f : formula) (N : cnf) (v : var) := FSAT f <-> SAT ([(true, v)] :: N). 
 
-Definition 
+Lemma tseytin'_nf_monotonic f nf v N nf' : tseytin' nf f = (v, N, nf') -> nf' >= nf. 
+Proof. 
+  revert nf v N nf'. induction f; cbn; intros nf v N nf' H; inv H; [lia | lia | | | ].
+  1-2: destruct (tseytin' nf f1) as ((rv1 & N1) & nfVar1) eqn:F1;
+    destruct (tseytin' nfVar1 f2) as ((rv2 & N2) & nfVar2) eqn:F2; 
+    apply IHf1 in F1; apply IHf2 in F2; inv H1; lia. 
+  destruct (tseytin' nf f) as ((rv' & N') & nfVar') eqn:H2.  
+  apply IHf in H2. inv H1. lia. 
+Qed.
+
+Hint Resolve varBound_cnf_monotonic.
+Hint Resolve varBound_cnf_app. 
+
+Hint Constructors varBound_cnf varBound_clause. 
+(*TODO: probably split up into compatibility lemmas for the different cases *)
+Lemma tseytin'_repr f nf v N nf' : varBound_formula nf f -> tseytin' nf f = (v, N, nf') -> varBound_cnf nf' N /\ v < nf' /\ formula_repr f N v. 
+Proof. 
+  revert nf nf' v N. induction f; cbn; intros. 
+  - inv H0. split; [ eauto | split; [lia | ]].
+    split; intros. 
+    + exists [v]; cbn. unfold satisfies. do 2 (cbn; rewrite Nat.eqb_refl). easy. 
+    + exists []; easy.
+  - inv H0. split; [eauto | split; [inv H; lia | ]]. split; intros [a H1]; exists a. 
+    + unfold FSAT.satisfies in H1. apply evalFormula_prim_iff in H1. unfold satisfies. cbn.
+      apply Bool.eqb_true_iff. now apply evalVar_in_iff. 
+    + unfold satisfies in H1. cbn in H1. apply Bool.eqb_prop in H1. apply evalVar_in_iff in H1. 
+      unfold FSAT.satisfies. now apply evalFormula_prim_iff. 
+  - destruct (tseytin' nf f1) as ((rv1 & N1) & nfVar1) eqn:F1.
+    destruct (tseytin' nfVar1 f2) as ((rv2 & N2) & nfVar2) eqn:F2. 
+    inv H. 
+    apply varBound_formula_monotonic with (n' := nf) in H3; [ | lia].
+    (*nfVar1 >= nf *)
+    specialize (tseytin'_nf_monotonic F1) as H7. 
+    specialize (tseytin'_nf_monotonic F2) as H8.
+    apply varBound_formula_monotonic with (n' := nfVar1) in H4; [ | lia].
+    specialize (IHf1 _ _ _ _ H3 F1) as (IH1 & IH2 & IH3).
+    specialize (IHf2 _ _ _ _ H4 F2) as (IH4 & IH5 & IH6).
+    inv H0. split; [ | split; [lia | ]].
+    + apply varBound_cnf_app; split; [ | apply varBound_cnf_app; split]; eauto 9.
+      eapply varBound_cnf_monotonic. 2: apply tseytinAnd_varBound. lia.
+    + split; intros [a H].
+      * exists (v :: rv1 :: rv2 :: a). unfold satisfies. 
+        unfold FSAT.satisfies in H; cbn in H. apply andb_true_iff in H as (He1 & He2).
+        (*better:app lemma *)
+        apply evalCnf_clause_iff. intros cl Hin. cbn in Hin. rewrite !in_app_iff in Hin. destruct_or Hin.
+        -- rewrite <- Hin. cbn. rewrite Nat.eqb_refl. easy.  
+        -- admit. (* use varBound to show that the new assignment is equivalent for the bounded cnf*)
+        -- admit. 
+        -- admit. 
+      * exists a. 
+        (*plan of attack: 
+          split along app/cons, derive that a[v] = true, use the equivalence for tseytinAnd, 
+          then the inductive hypotheses
+      *)
+Admitted. 
+
+Lemma tseytin_repr f v N : tseytin f = (v, N) -> formula_repr f N v. 
+Proof. 
+  unfold tseytin. destruct tseytin' as ((repVar & N1) & nfvar') eqn:H1.
+  intros H; inv H. eapply tseytin'_repr; [ | apply H1].
+  apply formula_bound_varBound.
+Qed.
+  
+
 
